Interface for MaxSat solvers

coq/Sat.v
@@ -1,14 +1,16 @@
+Require Import MSets.
+
 From RFXP Require Import CNF.
 
-Module Type SatSolver.
+Module Type SatSolverRaw.
 
     Variant ans := SAT (I : assignment nat) | UNSAT.
 
     Parameter solve : cnf nat -> ans.
 
-End SatSolver.
+End SatSolverRaw.
 
-Module Type IsCorrectSatSolver (Import Sat : SatSolver).
+Module Type IsCorrectSatSolver (Import Sat : SatSolverRaw).
 
     Axiom sat_correct : forall (c : cnf nat) (I : assignment nat),
         solve c = SAT I -> eval_cnf I c = true.
@@ -18,20 +20,171 @@ Module Type IsCorrectSatSolver (Import Sat : SatSolver).
 
 End IsCorrectSatSolver.
 
-Module Type CorrectSatSolver := SatSolver <+ IsCorrectSatSolver.
+Module Type SatSolver := SatSolverRaw <+ IsCorrectSatSolver.
 
 
-Module Type CCEncoder.
+Module Type CCEncoderRaw.
 
     Parameter encode : cnf_with_cc nat -> cnf nat.
 
-End CCEncoder.
+End CCEncoderRaw.
 
-Module Type IsCorrectCCEncoder (Import Enc : CCEncoder).
+Module Type IsCorrectCCEncoder (Import Enc : CCEncoderRaw).
 
     Axiom encode_correct : forall (c : cnf_with_cc nat) (I : assignment nat),
         eval_cnf I (encode c) = eval_cnf_with_cc I c.
 
 End IsCorrectCCEncoder.
 
-Module Type CorrectCCEncoder := CCEncoder <+ IsCorrectCCEncoder.
+Module Type CCEncoder := CCEncoderRaw <+ IsCorrectCCEncoder.
+
+
+Module Type MaxSatSolverRaw.
+
+    Declare Module S : Sets
+        with Definition E.t := nat
+        with Definition E.eq := @eq nat.
+
+    (* solve [hard clauses] [soft clauses] finds a maximally SAT set of soft clauses *)
+    Parameter solve : cnf nat -> cnf nat -> S.t * assignment nat.
+
+End MaxSatSolverRaw.
+
+Module MakeMaxSatEval (Import MSat : MaxSatSolverRaw).
+
+    Variant filt := include (X : S.t) | exclude (X : S.t).
+
+    Definition apply_filt (f : filt) :=
+        match f with
+        | include X => fun n => S.mem n X
+        | exclude X => fun n => negb (S.mem n X)
+        end.
+
+    Fixpoint filter_elts {A : Type} (f : filt) (c : list A) : nat -> list A -> list A :=
+        match c with
+        | nil => fun _ acc => acc
+        | cons cls c => fun n acc =>
+            if apply_filt f n then
+                filter_elts f c (S n) (cls :: acc)
+            else
+                filter_elts f c (S n) acc
+        end.
+
+    Definition make_cnf (f : filt) (c_hard c_soft : cnf nat) : cnf nat :=
+        filter_elts f c_soft 0 c_hard.
+
+    Definition maxsat_eval (I : assignment nat) (f : filt) (c_hard c_soft : cnf nat) :=
+        eval_cnf I (make_cnf f c_hard c_soft).
+
+
+    (* Specification of make_cnf *)
+
+    Lemma filter_elts_correct : forall {A : Type} (f : filt) (c acc : list A) (n : nat) (x : A),
+        List.In x (filter_elts f c n acc) <->
+            List.In x acc
+            \/ exists p, apply_filt f (n + p) = true /\ List.nth_error c p = Some x.
+    Proof.
+        intros A f c; induction c as [| y c IH ]; intros acc n x; split; intro H;
+            try (now left).
+        -   destruct H as [H | (p & H1 & H2)]; try assumption;
+            rewrite nth_error_nil in H2; discriminate.
+        -   simpl in H; destruct (apply_filt f n) eqn:Hf;
+            apply IH in H as [H | (p & H1 & H2)];
+                try (now left);
+                try (rewrite Nat_as_DT.add_succ_comm in H1; right; now exists (S p));
+            destruct H;
+                try (now left);
+            subst y; right; exists 0; now rewrite <- plus_n_O.
+        -   simpl; destruct (apply_filt f n) eqn:Hf; apply IH;
+            destruct H as [H | (p & H1 & H2)];
+                try (now left);
+                try (now (left; right));
+            destruct p;
+                try (now inversion H2; left; left);
+                try (simpl in H1; now rewrite <- plus_n_O, Hf in H1);
+            right; exists p; rewrite Nat_as_DT.add_succ_comm; now split.
+    Qed.
+
+
+    Theorem make_cnf_spec_include : forall (cls : clause nat) (X : S.t) (c_hard c_soft : cnf nat),
+        List.In cls (make_cnf (include X) c_hard c_soft) <->
+            List.In cls c_hard \/ exists n, S.In n X /\ List.nth_error c_soft n = Some cls.
+    Proof.
+        intros; unfold make_cnf; rewrite filter_elts_correct;
+        split; intros [H | H];
+            try (destruct H as (p & H1 & H2));
+            try (simpl in H1);
+            try (now left);
+            try (right; exists p; split);
+            try assumption;
+            try (now rewrite <- S.mem_spec);
+            try (simpl; now rewrite S.mem_spec).
+    Qed.
+
+    Theorem make_cnf_spec_exclude : forall (cls : clause nat) (X : S.t) (c_hard c_soft : cnf nat),
+        List.In cls (make_cnf (exclude X) c_hard c_soft) <->
+            List.In cls c_hard \/ exists n, ~ S.In n X /\ List.nth_error c_soft n = Some cls.
+    Proof.
+        intros; unfold make_cnf; rewrite filter_elts_correct;
+        split; intros [H | H];
+            try (destruct H as (p & H1 & H2));
+            try (simpl in H1);
+            try (now left);
+            try (right; exists p; split);
+            try assumption;
+            try (rewrite <- S.mem_spec; intro abs; now rewrite abs in H1);
+            try (simpl; apply eq_true_not_negb; intro abs; apply H1; now rewrite <- S.mem_spec).
+    Qed.
+
+    Theorem maxsat_eval_spec : forall (I : assignment nat) (f : filt) (c_hard c_soft : cnf nat),
+        maxsat_eval I f c_hard c_soft = eval_cnf I (make_cnf f c_hard c_soft).
+    Proof. reflexivity. Qed.
+
+
+    (* We may need to remove nats greater than the number of soft clauses in sets *)
+
+    Definition normalize : nat -> S.t -> S.t :=
+        fun m => S.filter (fun n => Nat.ltb n m).
+
+    Instance compatb : Proper (S.E.eq ==> S.E.eq ==> Logic.eq) (fun m n => Nat.ltb n m).
+        intros n p H; now rewrite H.
+    Defined.
+
+    Theorem normalize_spec : forall (n : nat) (X : S.t) (p : nat),
+        S.In p (normalize n X) <-> S.In p X /\ p < n.
+    Proof.
+        intros; unfold normalize; rewrite S.filter_spec;
+            try (now apply compatb);
+        split; intros (H1 & H2); split;
+            now destruct (Nat_as_DT.ltb_spec0 p n).
+    Qed.
+
+End MakeMaxSatEval.
+
+Module Type IsCorrectMaxSatSolver (Import MSat : MaxSatSolverRaw).
+
+    Module Import D := MakeMaxSatEval MSat.
+
+    Section Props.
+
+        Variables
+            (c_hard c_soft : cnf nat)
+            (Xout : S.t)
+            (Iin Iout : assignment nat).
+
+        Hypothesis result :
+            solve c_hard c_soft = (Xout, Iout).
+
+        Axiom mss_isSAT :
+            eval_cnf Iout (make_cnf (include Xout) c_hard c_soft) = true.
+
+        Axiom mss_isMax :
+            forall X I, S.Subset Xout X ->
+                eval_cnf I (make_cnf (include X) c_hard c_soft) = true ->
+                    S.Equal (normalize (length c_soft) X) (normalize (length c_soft) Xout).
+
+    End Props.
+
+End IsCorrectMaxSatSolver.
+
+Module Type MaxSatSolver := MaxSatSolverRaw <+ IsCorrectMaxSatSolver.
